examples/rel/Setoids.Crypto.Proof.fst
@@ -1,0 +1,368 @@
+module Setoids.Crypto.Proof
+open FStar.Bytes
+open FStar.UInt32
+open FStar.Map
+open Setoids
+open Setoids.Crypto
+open Setoids.Crypto.KEY
+open Setoids.Crypto.AE
+open Setoids.Crypto.ODH
+
+module DM = FStar.DependentMap
+
+#set-options "--z3rlimit 350 --max_fuel 0 --max_ifuel 0"
+let pkey n = share n
+let nonce = bytes
+
+abstract let pkae_state n aes = (ae_log #n aes * odh_state n) * key_state n
+
+let pkae_state_rel n aes = ((lo (ae_log #n aes)) ** (lo (odh_state n))) ** (lo (key_state n))
+
+#set-options "--z3rlimit 350 --max_fuel 0 --max_ifuel 1"
+let lift_ae_state #a (#arel:erel a) n aes (f:eff (lo (ae_log #n aes) ** lo (key_state n)) arel)
+  : eff (pkae_state_rel n aes) arel
+  = fun (t, ((ae_st, odh_st), key_st)) ->
+      match f (t, (ae_st, key_st)) with
+      | None, (ae_st', key_st'), t -> None, ((ae_st',odh_st), key_st'), t
+      | Some x, (ae_st', key_st'), t -> Some x, ((ae_st',odh_st), key_st'), t
+
+let lift_odh_state #a (#arel:erel a) n aes (f:eff (lo (odh_state n) ** lo (key_state n)) arel)
+  : eff (pkae_state_rel n aes) arel
+  = fun (t, ((ae_st, odh_st), key_st)) ->
+      match f (t, (odh_st, key_st)) with
+      | None, (odh_st', key_st'), t -> None, ((ae_st,odh_st'), key_st'), t
+      | Some x, (odh_st', key_st'), t -> Some x, ((ae_st,odh_st'), key_st'), t
+
+#set-options "--z3rlimit 350 --max_fuel 0 --max_ifuel 0"
+let ae_odh_sig n aes = sig_prod (odh_sig n) (ae_sig n aes)
+let ae_odh_module n aes = module_t (ae_odh_sig n aes)
+
+let pkae_gen_t n aes =
+  (lo unit)
+    ^--> eff_rel (((hi (ae_log #n aes)) ** (lo (odh_state n))) ** (lo (key_state n))) (lo (share n))
+
+let pkae_gen n aes (m:ae_odh_module n aes) : pkae_gen_t n aes
+  =
+  fun _ ->
+    let odh_gen : gen_dh_t n = get_oracle m (Inl GEN_DH) in
+    lift_odh_state n aes (odh_gen ())
+
+let pkae_enc_inputs n (aes:ae_scheme n) =
+  quatruple_rel
+    (lo (pkey n))
+    (lo (pkey n))
+    (lo nonce)
+    (lo (p:bytes{len p `lte` aes.max_plaintext_length}))
+
+let pkae_enc_t n aes =
+  pkae_enc_inputs n aes
+    ^--> eff_rel (pkae_state_rel n aes) (lo bytes)
+
+let pkae_enc n aes (m:ae_odh_module n aes) : pkae_enc_t n aes =
+  fun (sender_pk, receiver_pk, nonce, p) ->
+    let odh_exp : odh_t n = get_oracle m (Inl ODH) in
+    let ae_enc : enc_t n aes = get_oracle m (Inr ENC) in
+    h <-- lift_odh_state n aes (odh_exp (sender_pk, receiver_pk));
+    c <-- lift_ae_state n aes (ae_enc (p,nonce,h));
+    return #(pkae_state n aes) #bytes #(pkae_state_rel n aes) c
+
+let pkae_dec_inputs n (aes:ae_scheme n) =
+  quatruple_rel
+    (lo (pkey n))
+    (lo (pkey n))
+    (lo nonce)
+    (lo (c:bytes{len c `lte` aes.ciphertext_length aes.max_plaintext_length}))
+
+let pkae_dec_t n aes =
+  pkae_dec_inputs n aes
+    ^--> eff_rel (pkae_state_rel n aes) (option_rel (lo (p:bytes{len p `lte` aes.max_plaintext_length})))
+
+let pkae_dec n aes (m:ae_odh_module n aes) : pkae_dec_t n aes =
+  fun (sender_pk, receiver_pk, nonce, c) ->
+    let odh_exp : odh_t n = get_oracle m (Inl ODH) in
+    let ae_dec : dec_t n aes = get_oracle m (Inr DEC) in
+    h <-- lift_odh_state n aes (odh_exp (sender_pk, receiver_pk));
+    p <-- lift_ae_state n aes (ae_dec (c,nonce,h));
+    return p
+
+type pkae_labels =
+    | GEN
+    | ENC
+    | DEC
+
+#set-options "--z3rlimit 350 --max_fuel 0 --max_ifuel 1"
+let pkae_field_types n aes : pkae_labels -> Type =
+    function  GEN -> pkae_gen_t n aes
+            | ENC -> pkae_enc_t n aes
+            | DEC -> pkae_dec_t n aes
+
+let pkae_field_rels n aes : (l:pkae_labels -> erel (pkae_field_types n aes l)) =
+  function
+      GEN ->
+      arrow
+        (lo unit)
+        (eff_rel (((hi (ae_log #n aes)) ** (lo (odh_state n))) ** (lo (key_state n))) (lo (share n)))
+    | ENC ->
+      arrow
+        (pkae_enc_inputs n aes)
+        (eff_rel (pkae_state_rel n aes) (lo bytes))
+    | DEC ->
+      arrow
+        (pkae_dec_inputs n aes)
+        (eff_rel (pkae_state_rel n aes) (option_rel (lo (p:bytes{len p `lte` aes.max_plaintext_length}))))
+
+let pkae_sig (n:u32) (aes:ae_scheme n) = {
+    labels = pkae_labels;
+    ops = pkae_field_types n aes;
+    rels = pkae_field_rels n aes
+  }
+
+let pkae_module (n:u32) (aes:ae_scheme n) (m:ae_odh_module n aes) : module_t (pkae_sig n aes) =
+  DM.create #_ #(pkae_sig n aes).ops
+    (function GEN -> pkae_gen n aes m
+            | ENC -> pkae_enc n aes m
+            | DEC -> pkae_dec n aes m)
+
+let pkae_functor (n:u32) (aes:ae_scheme n)
+  : functor_t (sig_prod (odh_sig n) (ae_sig n aes)) (pkae_sig n aes)
+  = fun (m:module_t (sig_prod (odh_sig n) (ae_sig n aes))) ->
+      //pkae_module n aes m
+      admit()
+
+///     ID_WRITE
+///     -------- o KEY_0
+///     ID_READ
+let key0_id_composition n
+  : functor_t sig_unit (sig_prod (key_write_sig n) (key_read_sig n)) =
+  let id_composition =
+    functor_prod_shared_sig
+      (key_write_functor n)
+      (key_read_functor n) in
+  comp id_composition (KEY.key0_functor n)
+
+///     ID_WRITE
+///     -------- o KEY_1
+///     ID_READ
+let key1_id_composition n
+  : functor_t sig_unit (sig_prod (key_write_sig n) (key_read_sig n)) =
+  let id_composition =
+    functor_prod_shared_sig
+      (key_write_functor n)
+      (key_read_functor n) in
+  comp id_composition (KEY.key1_functor n)
+
+///   ODH
+///   ----
+///   AE_0
+let protocol0_composition n aes os
+  : functor_t (sig_prod (key_write_sig n) (key_read_sig n)) (sig_prod (odh_sig n) (ae_sig n aes)) =
+  functor_prod
+    (odh_functor n os)
+    (ae0_functor n aes)
+
+///   ODH
+///   ----
+///   AE_1
+let protocol1_composition n aes os
+  : functor_t (sig_prod (key_write_sig n) (key_read_sig n)) (sig_prod (odh_sig n) (ae_sig n aes)) =
+  functor_prod
+    (odh_functor n os)
+    (ae1_functor n aes)
+
+///         ODH    ID_WRITE
+///  PKAE o ---- o -------- o KEY_0
+///         AE_0   ID_READ
+let pkae0_composition n aes os
+  : functor_t sig_unit (pkae_sig n aes) =
+    let prot = comp (protocol0_composition n aes os) (key0_id_composition n) in
+    comp (pkae_functor n aes) prot
+
+///         ODH    ID_WRITE
+///  PKAE o ---- o -------- o KEY_1
+///         AE_0   ID_READ
+let pkae_intermediate_composition n aes os
+  : functor_t sig_unit (pkae_sig n aes) =
+    let prot = comp (protocol0_composition n aes os) (key1_id_composition n) in
+    comp (pkae_functor n aes) prot
+
+///         ODH    ID_WRITE
+///  PKAE o ---- o -------- o KEY_1
+///         AE_1   ID_READ
+let pkae1_composition n aes os
+  : functor_t sig_unit (pkae_sig n aes) =
+    let prot = comp (protocol1_composition n aes os) (key0_id_composition n) in
+    comp (pkae_functor n aes) prot
+
+let pkae_rel n aes : per (functor_t sig_unit (pkae_sig n aes))  = fun (pkae0:functor_t sig_unit (pkae_sig n aes)) (pkae1:functor_t sig_unit (pkae_sig n aes)) ->
+  let pkae0_module = pkae0 mod_unit in
+  let pkae1_module = pkae1 mod_unit in
+  sig_rel' (pkae_sig n aes) pkae0_module pkae1_module
+
+/// The following doesn't verify. I'm just trying to hint at how I would imagine the proof would go.
+
+/// Proof:
+/// Assumptions:
+/// ODH o ID_WRITE            ODH o ID_WRITE
+/// -------------- o KEY_0 =  -------------- o KEY_1
+///    ID_READ                    ID_READ
+
+///    ID_WRITE                     ID_WRITE
+/// ---------------- o KEY_1 =  ---------------- o KEY_1
+///  AE_0 o ID_READ              AE_1 o ID_READ
+///
+/// Goal: Show that we can instantiate an eq instance with pkae0 and pkae1
+/// Note, that for the full cryptographic proof, we would have to show `Perfect`
+/// equivalence with the actual PKAE security notion, which I have not yet
+/// encoded. However, that should be trivial, once we have make the following
+/// work.
+
+/// First step: pull ODH assumption to the right and make sure the result is
+/// still equal. Then idealize ODH and pull it back to the left.
+///         ODH    ID_WRITE
+///  PKAE o ---- o -------- o KEY_0
+///         AE_0   ID_READ
+/// to
+///         ID_ODH     ODH o ID_WRITE
+///  PKAE o ------ o ----------------- o KEY_0
+///         AE_0         ID_READ
+/// to
+///         ID_ODH     ODH o ID_WRITE
+///  PKAE o ------ o ----------------- o KEY_1
+///         AE_0         ID_READ
+/// to
+///         ODH    ID_WRITE
+///  PKAE o ---- o -------- o KEY_1
+///         AE_0   ID_READ
+let step1_left_side n aes =
+  comp (pkae_functor n aes)
+       (functor_prod
+         id_func
+         (ae0_functor n aes))
+
+/// Second step: pull AE assumption to the right and make sure the result is
+/// still equal. Then idealize AE and pull it back to the left.
+///         ODH    ID_WRITE
+///  PKAE o ---- o -------- o KEY_1
+///         AE_0   ID_READ
+/// to
+///         ODH        ID_WRITE
+///  PKAE o ---- o ----------------- o KEY_1
+///         ID_AE    AE_0 o ID_READ
+/// to
+///         ODH        ID_WRITE
+///  PKAE o ---- o ----------------- o KEY_1
+///         ID_AE    AE_1 o ID_READ
+/// to
+///         ODH    ID_WRITE
+///  PKAE o ---- o -------- o KEY_1
+///         AE_1   ID_READ
+let step2_left_side n os aes =
+  comp
+    (pkae_functor n aes)
+    (functor_prod (odh_functor n os) id_func)
+
+let ae_step_eps n os aes = (eps_trans (step2_left_side n os aes) (ae_eps n aes))
+let odh_step_eps n aes = (eps_trans (step1_left_side n aes) (odh_eps n))
+let eps_sum n os aes = sum (ae_step_eps n os aes) (odh_step_eps n aes)
+
+#set-options "--z3rlimit 350 --max_fuel 0 --max_ifuel 0"
+let pkae_proof (n:u32) (aes:ae_scheme n) (os:odh_scheme n)
+  : eq (pkae_rel n aes)
+       (eps_sum n os aes)
+       (pkae0_composition n aes os)
+       (pkae1_composition n aes os) =
+  // Prove here, that pulling ODH to the right doesn't change anything.
+  let step1a_eq
+  : eq
+    (pkae_rel n aes)
+    (eps_z)
+    (pkae0_composition n aes os)
+    (comp
+      (step1_left_side n aes)
+      (odh_game0 n os))
+    =
+    Perfect #_ #_ #(pkae_rel n aes)
+      (pkae0_composition n aes os)
+      (comp
+        (step1_left_side n aes)
+        (odh_game0 n os))
+      ()
+  in
+  // Now apply the ODH assumption via the Ctx rule.
+  let step1b_eq
+  : eq
+    (pkae_rel n aes)
+    (odh_step_eps n aes)
+    (pkae0_composition n aes os)
+    (comp
+      (step1_left_side n aes)
+      (odh_game1 n os))
+    =
+    Trans
+      step1a_eq
+      (Ctx #_ #_ #(pkae_rel n aes)
+        (odh_assumption n os)
+        (step1_left_side n aes))
+  in
+  // Finish the first step by pulling ODH to the left again. Note, that the KEY package is now idealized (KEY_0 -> KEY_1)
+  // and prove again, that nothing changes by pulling ODH back to the left (now with KEY_1 instead of KEY_0).
+  let step1_final_eq
+  : eq
+    (pkae_rel n aes)
+    (odh_step_eps n aes)
+    (pkae0_composition n aes os)
+    (pkae_intermediate_composition n aes os)
+  =
+    Trans
+      step1b_eq
+      (Perfect #_ #_ #(pkae_rel n aes)
+        (comp
+          (step1_left_side n aes)
+          (odh_game1 n os))
+        (pkae_intermediate_composition n aes os)
+        ())
+  in
+  let step2a_eq
+  : eq
+    (pkae_rel n aes)
+    (odh_step_eps n aes)
+    (pkae0_composition n aes os)
+    (comp
+      (step2_left_side n os aes)
+      (ae_game0 n aes))
+  =
+    Trans
+      step1_final_eq
+      (Perfect #_ #_ #(pkae_rel n aes)
+        (pkae_intermediate_composition n aes os)
+        (comp
+          (step2_left_side n os aes)
+          (ae_game0 n aes))
+        ())
+  in
+  // Now apply the AE assumption via the Ctx rule.
+  let step2b_eq
+  : eq
+    (pkae_rel n aes)
+    (eps_sum n os aes)
+    (pkae0_composition n aes os)
+    (comp
+      (step2_left_side n os aes)
+      (ae_game1 n aes))
+  =
+    Trans
+      step2a_eq
+      (Ctx #_ #_ #(pkae_rel n aes)
+        (ae_assumption n aes)
+        (step2_left_side n os aes))
+  in
+  // Finish the first step by pulling ODH to the left again. Note, that the KEY package is now idealized (KEY_0 -> KEY_1)
+  // and prove again, that nothing changes by pulling ODH back to the left (now with KEY_1 instead of KEY_0).
+  Trans
+    step2b_eq
+    (Perfect #_ #_ #(pkae_rel n aes)
+      (comp
+        (step2_left_side n os aes)
+        (ae_game1 n aes))
+      (pkae1_composition n aes os)
+      ())
